@prefix ex: <http://www.example.org#> .
@prefix dqv: <http://www.w3.org/ns/dqv#> .
@prefix owl: <http://www.w3.org/2002/07/owl#> .
@prefix rdf: <http://www.w3.org/1999/02/22-rdf-syntax-ns#> .
@prefix xml: <http://www.w3.org/XML/1998/namespace> .
@prefix xsd: <http://www.w3.org/2001/XMLSchema#> .
@prefix prov: <http://www.w3.org/ns/prov#> .
@prefix rdfs: <http://www.w3.org/2000/01/rdf-schema#> .
@prefix skos: <http://www.w3.org/2004/02/skos/core#> .
@prefix spin: <http://spinrdf.org/spin#> .
@prefix dcterms: <http://purl.org/dc/terms/> .

_:genid879806159 a owl:Ontology .
# 
# 
# #################################################################
# #
# #    Annotation properties
# #
# #################################################################
# 
# 
# http://www.example.org#flags

ex:flags a owl:AnnotationProperty .
# 
# http://www.example.org#hasMetricType

ex:hasMetricType a owl:AnnotationProperty .
# 
# http://www.w3.org/1999/02/22-rdf-syntax-ns#about

rdf:about a owl:AnnotationProperty .
# 
# http://www.w3.org/2004/02/skos/core#definition

skos:definition a owl:AnnotationProperty .
# 
# http://www.w3.org/2004/02/skos/core#note

skos:note a owl:AnnotationProperty .
# 
# http://www.w3.org/2004/02/skos/core#prefLabel

skos:prefLabel a owl:AnnotationProperty .
# 
# http://www.w3.org/ns/dqv#expectedDataType

dqv:expectedDataType a owl:AnnotationProperty .
# 
# http://www.w3.org/ns/dqv#inCategory

dqv:inCategory a owl:AnnotationProperty .
# 
# http://www.w3.org/ns/dqv#inDimension

dqv:inDimension a owl:AnnotationProperty .
# 
# 
# 
# #################################################################
# #
# #    Object Properties
# #
# #################################################################
# 
# 
# http://www.example.org#Flags

ex:Flags a owl:ObjectProperty .
# 
# http://www.example.org#hasMeasurement

ex:hasMeasurement a owl:ObjectProperty ;
	owl:inverseOf dqv:isMeasurementOf .

dqv:isMeasurementOf a owl:ObjectProperty .
# 
# http://www.example.org#hasPart

ex:hasPart a owl:ObjectProperty ;
	owl:inverseOf ex:isPartOf .
# 
# http://www.example.org#hasPrimaryDataset

ex:hasPrimaryDataset a owl:ObjectProperty .
# 
# http://www.example.org#hasShape

ex:hasShape a owl:ObjectProperty .
# 
# http://www.example.org#hasTargetDataset

ex:hasTargetDataset a owl:ObjectProperty .
# 
# http://www.example.org#isPartOf

ex:isPartOf a owl:ObjectProperty .
# 
# http://www.w3.org/ns/dqv#isMeasurementOf
# 
# 
# 
# #################################################################
# #
# #    Classes
# #
# #################################################################
# 
# 
# http://www.example.org#DataQuality

ex:DataQuality a owl:Class ;
	rdfs:subClassOf ex:Quality ;
	rdfs:comment "Encompasses the quality of information in the dataset."@en , "Metrics of type Dataquality (including the subclasses of ex:Dataquality) are generally measured on a dataset, whereas metrics of type Dataset quality are measured on a specific distribution. "@en .
# 
# http://www.example.org#DatasetQuality

ex:DatasetQuality a owl:Class ;
	rdfs:subClassOf ex:Quality ;
	rdfs:comment "Encompasses the quality of the dataset or source, instead of the information stored in the dataset."@en .
# 
# http://www.example.org#InstanceQuality

ex:InstanceQuality a owl:Class ;
	rdfs:subClassOf ex:DataQuality ;
	rdfs:comment "Encompasses the quality of the instances of which the data consists. Measurements regarding metrics of this type, also annotate related instances"@en .
# 
# http://www.example.org#Quality

ex:Quality a owl:Class ;
	rdf:about "https://goo.gl/gbS6Lc" ;
	rdfs:comment "Quality is a very ambiguous term. In the context of this graph, we refer to the following breakdown of quality."@en .
# 
# http://www.example.org#SchemaQuality

ex:SchemaQuality a owl:Class ;
	rdfs:subClassOf ex:DataQuality ;
	rdfs:comment "Encompasses quality of the schema on top of the data. Measurements regarding metrics of this type, also annotate related classes and properties."@en .
# 
# http://www.w3.org/ns/dqv#Dimension

dqv:Dimension a owl:Class .
# 
# http://www.w3.org/ns/dqv#Metric

dqv:Metric a owl:Class .
# 
# http://www.w3.org/ns/dqv#QualityMeasurementDataset

dqv:QualityMeasurementDataset a owl:Class .
# 
# 
# 
# #################################################################
# #
# #    Individuals
# #
# #################################################################
# 
# 
# http://www.example.org#QualityMeasurementDataset

ex:QualityMeasurementDataset a owl:NamedIndividual , dqv:QualityMeasurementDataset ;
	skos:prefLabel "Quality Measurement Dataset"@en .
# 
# http://www.example.org#RDFdumpavailability

ex:RDFdumpavailability a owl:NamedIndividual , dqv:Metric ;
	ex:hasMetricType ex:DatasetQuality ;
	skos:definition "Checking whether accessible/downloadable RDF dumps are provided. "@en ;
	skos:prefLabel "RDF Dump Availability"@en ;
	dqv:expectedDataType xsd:boolean ;
	dqv:inDimension ex:availability .
# 
# http://www.example.org#SPARQLendpointaccessibility

ex:SPARQLendpointaccessibility a owl:NamedIndividual , dqv:Metric ;
	ex:hasMetricType ex:DatasetQuality ;
	skos:definition "Checking whether a working SPARQL endpoint is present. No differentiation is made based on the quality of the response for this measure (either based on time or content)."@en ;
	skos:prefLabel "SPARQL Endpoint Accessibility"@en ;
	dqv:expectedDataType xsd:boolean ;
	dqv:inDimension ex:availability .
# 
# http://www.example.org#URIlength

ex:URIlength a owl:NamedIndividual , dqv:Metric ;
	ex:hasMetricType ex:DatasetQuality ;
	skos:definition "URIs should be readable and concise. Making sure there is no redundant information is present in the URI makes it more easily understood and de-referenced."@en ;
	skos:prefLabel "URIs Length"@en ;
	dqv:expectedDataType xsd:boolean ;
	dqv:inDimension ex:representationalConciseness .
# 
# http://www.example.org#accuracy

ex:accuracy a owl:NamedIndividual , dqv:Dimension ;
	skos:definition "Degree of correctness and precision with which information in an information system represents states of the real world. Can be divided into semantic (correctness in regard to real world values) and syntactic (correctness in regard to its definition domain) accuracy."@en ;
	skos:prefLabel "Accuracy"@en ;
	dqv:inCategory ex:intrinsic .
# 
# http://www.example.org#ambiguousinstances

ex:ambiguousinstances a owl:NamedIndividual , dqv:Metric ;
	ex:hasMetricType ex:InstanceQuality ;
	skos:definition "Instances mapping to more than one real-world object, resulting in multiple possible interpretations."@en ;
	skos:prefLabel "Ambiguous Instances"@en ;
	dqv:expectedDataType xsd:integer ;
	dqv:inDimension ex:consistency .
# 
# http://www.example.org#amountOfData

ex:amountOfData a owl:NamedIndividual , dqv:Dimension ;
	skos:definition "Measures the appropriateness of the volume and quantity of data for a given task. "@en ;
	skos:prefLabel "Amount of Data"@en ;
	dqv:inCategory ex:contextual .
# 
# http://www.example.org#amountofclasses

ex:amountofclasses a owl:NamedIndividual , dqv:Metric ;
	ex:hasMetricType ex:SchemaQuality ;
	skos:definition "The amount of distinct classes in the dataset."@en ;
	skos:prefLabel "Amount of Classes"@en ;
	dqv:expectedDataType xsd:integer ;
	dqv:inDimension ex:completeness .
# 
# http://www.example.org#amountofproperties

ex:amountofproperties a owl:NamedIndividual , dqv:Metric ;
	ex:hasMetricType ex:SchemaQuality ;
	skos:definition "The amount of distinct properties in the dataset."@en ;
	skos:prefLabel "Amount of Properties"@en ;
	dqv:expectedDataType xsd:integer ;
	dqv:inDimension ex:completeness .
# 
# http://www.example.org#amountofresources

ex:amountofresources a owl:NamedIndividual , dqv:Metric ;
	ex:hasMetricType ex:DataQuality ;
	skos:definition "The amount of resources in the dataset."@en ;
	skos:prefLabel "Amount of Resources"@en ;
	dqv:expectedDataType xsd:integer ;
	dqv:inDimension ex:completeness .
# 
# http://www.example.org#amountoftriples

ex:amountoftriples a owl:NamedIndividual , dqv:Metric ;
	ex:hasMetricType ex:DatasetQuality ;
	skos:definition "The amount of triples in the dataset."@en ;
	skos:prefLabel "Amount of Triples"@en ;
	dqv:expectedDataType xsd:integer ;
	dqv:inDimension ex:completeness .
# 
# http://www.example.org#attributeAccuracy

ex:attributeAccuracy a owl:NamedIndividual , dqv:Metric ;
	ex:hasMetricType ex:InstanceQuality ;
	skos:definition "Degree in which measurements are correct, or how precise the measurement was conducted. For instance with Geo spatial data, measurements can be done in meters or millimeters. "@en ;
	skos:prefLabel "Attribute Accuracy"@en ;
	dqv:expectedDataType rdfs:Literal ;
	dqv:inDimension ex:accuracy .
# 
# http://www.example.org#availability

ex:availability a owl:NamedIndividual , dqv:Dimension ;
	skos:definition "Availability of a dataset is the extent to which data (or some portion of it) is present, obtainable and ready for use."@en ;
	skos:prefLabel "Availability"@en ;
	dqv:inCategory ex:accessibility .
# 
# http://www.example.org#believability

ex:believability a owl:NamedIndividual , dqv:Dimension ;
	skos:definition "The degree to which the data is considered true and correct."@en ;
	skos:prefLabel "Believability"@en ;
	dqv:inCategory ex:contextual , ex:trust .
# 
# http://www.example.org#blanknodes

ex:blanknodes a owl:NamedIndividual , dqv:Metric ;
	ex:hasMetricType ex:DataQuality ;
	skos:definition "Measures the percentage of blank nodes among the total number of URIs. "@en ;
	skos:prefLabel "Blank Nodes"@en ;
	dqv:expectedDataType xsd:float ;
	dqv:inDimension ex:interpretability .
# 
# http://www.example.org#community

ex:community a owl:NamedIndividual , dqv:Metric ;
	ex:hasMetricType ex:DatasetQuality ;
	skos:definition "Providing message boards and mailing list can be used to actively improve, and help users understand and query the dataset. This metric measure the presence and use of such mechanism. A neglected message board might indicate that the dataset is no longer updated. The value of this metric is True only when message boards and/or mailing list are provided and used."@en ;
	skos:prefLabel "Community"@en ;
	dqv:expectedDataType xsd:boolean ;
	dqv:inDimension ex:understandability .
# 
# http://www.example.org#completeness

ex:completeness a owl:NamedIndividual , dqv:Dimension ;
	skos:definition "The degree to which all required information is present in a dataset. completeness can be determined on three levels, 1) schema, also ontology completeness, 2) property completeness, measure of missing values and 3) population completeness, percentage of real world objects represented in the dataset."@en ;
	skos:prefLabel "Completeness"@en ;
	dqv:inCategory ex:contextual .
# 
# http://www.example.org#conciseness

ex:conciseness a owl:NamedIndividual , dqv:Dimension ;
	skos:definition "Conciseness concerns the presence of redundant information in the dataset, either at schema level or instance level."@en ;
	skos:prefLabel "Conciseness"@en ;
	dqv:inCategory ex:intrinsic .
# 
# http://www.example.org#consistency

ex:consistency a owl:NamedIndividual , dqv:Dimension ;
	skos:definition "A dataset is consistent if it is free of conflicting information with respect to particular knowledge representation and inference mechanisms."@en ;
	skos:prefLabel "Concistency"@en ;
	dqv:inCategory ex:intrinsic .
# 
# http://www.example.org#contentnegotiation

ex:contentnegotiation a owl:NamedIndividual , dqv:Metric ;
	ex:hasMetricType ex:DatasetQuality ;
	skos:definition "Checking whether data can be retrieved in accepted formats and languages by adding a corresponding accept-header to an HTTP request"@en ;
	skos:prefLabel "Content Negotiation"@en ;
	dqv:expectedDataType xsd:boolean ;
	dqv:inDimension ex:versatility .
# 
# http://www.example.org#contenttype

ex:contenttype a owl:NamedIndividual , dqv:Metric ;
	ex:hasMetricType ex:DatasetQuality ;
	skos:definition "Meta data attached to the http request when dereferencing a URI in a browser, can include a 'content type'. User agents can use this to quickly identify pages containing RDF. "@en ;
	skos:prefLabel "Content Type"@en ;
	dqv:expectedDataType xsd:string ;
	dqv:inDimension ex:availability .
# 
# http://www.example.org#copyright

ex:copyright a owl:NamedIndividual , dqv:Metric ;
	ex:hasMetricType ex:DatasetQuality ;
	skos:definition "Detection of whether the work is attributed in the same way as specified by the author or licensor. Share-alike and copyleft roughly imply that the work in question should be licensed similarly as referenced sources. The work in question can also specify share-alike and copyleft requirements."@en ;
	skos:prefLabel "Copyright"@en ;
	dqv:expectedDataType xsd:boolean ;
	dqv:inDimension ex:licencing .
# 
# http://www.example.org#coverage

ex:coverage a owl:NamedIndividual , dqv:Metric ;
	ex:hasPart ex:descriptiveness , ex:scope ;
	ex:hasMetricType ex:InstanceQuality ;
	skos:definition "Coverage measures the scope of the dataset as the number of entities represented and the descriptiveness as the number of properties known for each entity."@en ;
	skos:prefLabel "Coverage"@en ;
	dqv:inDimension ex:amountOfData .
# 
# http://www.example.org#currency

ex:currency a owl:NamedIndividual , dqv:Dimension ;
	skos:definition "Measures the speed with with data values are updates after the real-world values change."@en ;
	skos:prefLabel "Currency"@en ;
	dqv:inCategory ex:datasetdynamicity .
# 
# http://www.example.org#currencyofdataset

ex:currencyofdataset a owl:NamedIndividual , dqv:Metric ;
	ex:hasMetricType ex:DataQuality ;
	skos:definition "Measures how current the data is."@en ;
	skos:prefLabel "Currency of Dataset"@en ;
	dqv:expectedDataType xsd:float ;
	dqv:inDimension ex:currency .
# 
# http://www.example.org#currencyofdatasetcomparison

ex:currencyofdatasetcomparison a owl:NamedIndividual , dqv:Metric ;
	ex:hasMetricType ex:DatasetQuality ;
	skos:definition "Measure the difference between the primary and Target dataset in terms of currency. "@en ;
	skos:prefLabel "Currency of Dataset Comparison"@en ;
	dqv:expectedDataType xsd:dayTimeDuration ;
	dqv:inDimension ex:currency .
# 
# http://www.example.org#dataaccesssecurity

ex:dataaccesssecurity a owl:NamedIndividual , dqv:Metric ;
	ex:hasMetricType ex:DatasetQuality ;
	skos:definition "Use of login credentials or use of SSL or SSH."@en ;
	skos:prefLabel "Data Access Security"@en ;
	dqv:expectedDataType xsd:boolean ;
	dqv:inDimension ex:security .
# 
# http://www.example.org#dataofproprietarynature

ex:dataofproprietarynature a owl:NamedIndividual , dqv:Metric ;
	ex:hasMetricType ex:DatasetQuality ;
	skos:definition "Data only available to specific users is of proprietary nature. Even if only parts of the data is hidden from access for the outside world (possibly due to a sensitive nature of the data), this metric should be scored 'False'"@en ;
	skos:prefLabel "Data of Proprietary Nature"@en ;
	dqv:expectedDataType xsd:boolean ;
	dqv:inDimension ex:security .
# 
# http://www.example.org#datasetlanguage

ex:datasetlanguage a owl:NamedIndividual , dqv:Metric ;
	ex:hasMetricType ex:DatasetQuality ;
	skos:definition "Checking whether data is available in different languages. For some purposes one would require the Target dataset to be in the same language as the primary dataset or at least another language that is sufficiently understood by the target users. This metric measures the amount of languages the dataset is published in. "@en ;
	skos:prefLabel "Dataset Language"@en ;
	dqv:expectedDataType xsd:language ;
	dqv:inDimension ex:versatility .
# 
# http://www.example.org#de-referencability

ex:de-referencability a owl:NamedIndividual , dqv:Metric ;
	ex:hasMetricType ex:DatasetQuality ;
	skos:definition "When a URI can not be properly dereferenced through a web browser and thus returns a server or client  error, this is seen as a de-referencability issue."@en ;
	skos:note "Each URI that turned out to be not dereferencable, should be annotated. The proposed method is by means of the triple: <subject> ex:isDereferencable 'False' "@en ;
	skos:prefLabel "De-referencability"@en ;
	dqv:expectedDataType xsd:float ;
	dqv:inDimension ex:availability .
# 
# http://www.example.org#de-referencedbacklinks

ex:de-referencedbacklinks a owl:NamedIndividual , dqv:Metric ;
	ex:hasMetricType ex:DatasetQuality ;
	skos:definition "detection of all local in-links or back-links: locally available triples in which the resource URI appears as an object, in the dereferenced document returned for the given resource."@en ;
	skos:prefLabel "De-referenced Back-Links"@en ;
	dqv:expectedDataType xsd:float ;
	dqv:inDimension ex:availability .
# 
# http://www.example.org#de-referencedforwardlinks

ex:de-referencedforwardlinks a owl:NamedIndividual , dqv:Metric ;
	ex:hasMetricType ex:DatasetQuality ;
	skos:definition "Detection of all forward links: locally known triples where the local URI is mentioned in the subject"@en ;
	skos:prefLabel "De-referenced Forward-Links"@en ;
	dqv:expectedDataType xsd:float ;
	dqv:inDimension ex:availability .
# 
# http://www.example.org#deprecatedclasses

ex:deprecatedclasses a owl:NamedIndividual , dqv:Metric ;
	ex:hasMetricType ex:SchemaQuality ;
	skos:definition "Count the occurences of classes of type owl:DeprecatedClass"@en ;
	skos:prefLabel "Deprecated Classes"@en ;
	dqv:expectedDataType xsd:integer ;
	dqv:inDimension ex:consistency .
# 
# http://www.example.org#deprecatedproperties

ex:deprecatedproperties a owl:NamedIndividual , dqv:Metric ;
	ex:hasMetricType ex:SchemaQuality ;
	skos:definition "Count the occurences of classes of type owl:DeprecatedProperty"@en ;
	skos:prefLabel "Deprecated Properties"@en ;
	dqv:expectedDataType xsd:integer ;
	dqv:inDimension ex:consistency .
# 
# http://www.example.org#descriptiveness

ex:descriptiveness a owl:NamedIndividual ;
	ex:isPartOf ex:coverage ;
	skos:definition "Measure the average number of attributes known for entities"@en ;
	skos:prefLabel "Descriptiveness"@en ;
	dqv:expectedDataType xsd:float .
# 
# http://www.example.org#disjointclasses

ex:disjointclasses a owl:NamedIndividual , dqv:Metric ;
	ex:hasMetricType ex:InstanceQuality ;
	skos:definition "entities (inferred to be) part of two disjoint classes. This metric measures the percentage of entities where this is the case."@en ;
	skos:prefLabel "Disjoint Classes"@en ;
	dqv:expectedDataType xsd:integer ;
	dqv:inDimension ex:consistency .
# 
# http://www.example.org#duplicateinstance

ex:duplicateinstance a owl:NamedIndividual , dqv:Metric ;
	ex:hasMetricType ex:InstanceQuality ;
	skos:definition "Measures the amount of duplicate instances"@en ;
	skos:prefLabel "Duplicate Instance"@en ;
	dqv:expectedDataType xsd:integer ;
	dqv:inDimension ex:conciseness .
# 
# http://www.example.org#exemplarySPARQL

ex:exemplarySPARQL a owl:NamedIndividual , dqv:Metric ;
	ex:hasMetricType ex:DatasetQuality ;
	skos:definition "As with the exemplary URIs, exemplary SPARQL queries provide insight as to how the dataset can be queried. "@en ;
	skos:prefLabel "Exemplary SPARQL"@en ;
	dqv:expectedDataType xsd:boolean ;
	dqv:inDimension ex:understandability .
# 
# http://www.example.org#exemplaryURIs

ex:exemplaryURIs a owl:NamedIndividual , dqv:Metric ;
	ex:hasMetricType ex:DatasetQuality ;
	skos:definition "Detecting whether the URI patterns are provided"@en ;
	skos:prefLabel "Exemplary URIs"@en ;
	dqv:expectedDataType <http://www.w3.org/2001/XMLSchema#> ;
	dqv:inDimension ex:understandability .
# 
# http://www.example.org#extensionalconciseness

ex:extensionalconciseness a owl:NamedIndividual , dqv:Metric ;
	ex:hasMetricType ex:InstanceQuality ;
	skos:definition "Measures the percentage of unique objects in the dataset. "@en ;
	skos:prefLabel "Extensional Conciseness"@en ;
	dqv:expectedDataType xsd:float ;
	dqv:inDimension ex:conciseness .
# 
# http://www.example.org#frequencyofchange

ex:frequencyofchange a owl:NamedIndividual , dqv:Metric ;
	ex:hasMetricType ex:DatasetQuality ;
	skos:definition "Refer to the changefrequency attribute in a Semantic Sitemap for value of the frequency or updates of a data source"@en ;
	skos:note "expected datatype range is limited to the following: [always, hourly, daily, weekly, monthly, yearly, never]"@en ;
	skos:prefLabel "Frequency of Change"@en ;
	dqv:expectedDataType xsd:string ;
	dqv:inDimension ex:volatility .
# 
# http://www.example.org#geometryblanknode

ex:geometryblanknode a owl:NamedIndividual , dqv:Metric ;
	ex:hasMetricType ex:InstanceQuality ;
	skos:definition "The dataset contains instances representing all the 'buurten' (neighbourhoods) in the Netherlands. Each of these should be accompanied by a geometry representing the geographical area considered a specific neighbourhood. Best practices mandate that a geometry should be attached to a blank node, which is in turn linked to the neighbourhood."@en ;
	skos:prefLabel "Geometry Blank Node"@en ;
	dqv:expectedDataType xsd:boolean ;
	dqv:inDimension ex:Interpretability .
# 
# http://www.example.org#human-readablelabelling

ex:human-readablelabelling a owl:NamedIndividual , dqv:Metric ;
	ex:hasMetricType ex:DataQuality ;
	skos:definition "percentage of resources containing a human readable label. For instance by means of an rdfs:label or rdfs:comment. Other vocabularies also offer labelling functions such as skos:preflabel or skos:note."@en ;
	skos:prefLabel "Human-Readable Labelling"@en ;
	dqv:expectedDataType xsd:float ;
	dqv:inDimension ex:understandability .
# 
# http://www.example.org#human-readablelicence

ex:human-readablelicence a owl:NamedIndividual , dqv:Metric ;
	ex:hasMetricType ex:DatasetQuality ;
	skos:definition "Detection of a license in the documentation of the dataset or its source"@en ;
	skos:prefLabel "Human-Readable Licence"@en ;
	dqv:expectedDataType xsd:boolean ;
	dqv:inDimension ex:licencing .
# 
# http://www.example.org#inaccuratefacts

ex:inaccuratefacts a owl:NamedIndividual , dqv:Metric ;
	ex:hasMetricType ex:InstanceQuality ;
	skos:definition "Check for inconsistencies by comparing the data to that of other sources. The metric measures the amount of facts deemed correct, by lack of evidence against the fact."@en ;
	skos:prefLabel "Inaccurate Facts"@en ;
	dqv:expectedDataType xsd:integer ;
	dqv:inDimension ex:accuracy .
# 
# http://www.example.org#inaccuratevalues

ex:inaccuratevalues a owl:NamedIndividual , dqv:Metric ;
	ex:hasMetricType ex:InstanceQuality ;
	skos:definition "This metric measures the amount of inaccurate values by using functional dependencies rules between the values of two or more different predicates. A functional dependency is a constraint between different properties of an instance, in the case of linked data. the underlying concept is that if one value for property X of an instance always co-occurs with a precisely one value for property Y, then it can be said that X determines the value of Y. "@en ;
	skos:prefLabel "Inaccurate Values"@en ;
	dqv:expectedDataType xsd:integer ;
	dqv:inDimension ex:accuracy .
# 
# http://www.example.org#incompatibledatatyperange

ex:incompatibledatatyperange a owl:NamedIndividual , dqv:Metric ;
	ex:hasMetricType ex:InstanceQuality ;
	skos:definition "Detection of ill-typed literals which do not abide by the lexical syntax for their respective datatype."@en ;
	skos:prefLabel "Incompatible Datatype Range"@en ;
	dqv:expectedDataType xsd:integer ;
	dqv:inDimension ex:accuracy .
# 
# http://www.example.org#indicativeness

ex:indicativeness a owl:NamedIndividual , dqv:Metric ;
	ex:hasMetricType ex:Quality ;
	skos:definition "Denotes the amount of metrics measured in the form of a grade between 1 and 10."@en ;
	skos:prefLabel "Indicativeness"@en ;
	dqv:expectedDataType xsd:integer ;
	dqv:inDimension ex:verifiability .
# 
# http://www.example.org#instanceenrichment

ex:instanceenrichment a owl:NamedIndividual , dqv:Metric ;
	ex:hasMetricType ex:InstanceQuality ;
	skos:definition "Percentage of attributes gained by interlinking and owl:sameAs relations."@en ;
	skos:prefLabel "Instance Enrichment"@en ;
	dqv:expectedDataType xsd:float ;
	dqv:inDimension ex:interlinking .
# 
# http://www.example.org#intentionalconciseness

ex:intentionalconciseness a owl:NamedIndividual , dqv:Metric ;
	ex:hasMetricType ex:InstanceQuality ;
	skos:definition "Measures the percentage of unique attributes in the dataset. "@en ;
	skos:prefLabel "Intentional Conciseness"@en ;
	dqv:expectedDataType xsd:float ;
	dqv:inDimension ex:consiceness .
# 
# http://www.example.org#interlinking

ex:interlinking a owl:NamedIndividual , dqv:Dimension ;
	skos:definition "Interlinking involves creating triples where the object and subject refer to the same concept and the object and subject can either originate from different datasets, of the same dataset. The interlinking dimension refers to the extend where this the case."@en ;
	skos:prefLabel "Interlinking"@en ;
	dqv:inCategory ex:accessibility .
# 
# http://www.example.org#interlinkingcompleteness

ex:interlinkingcompleteness a owl:NamedIndividual , dqv:Metric ;
	ex:hasMetricType ex:DatasetQuality ;
	skos:definition "Interlinking completeness measures the amount of instances that are interlinked in respect to the total amount of instances."@en ;
	skos:note "Metric can only be measured after interlinking."@en ;
	skos:prefLabel "Interlinking Completeness"@en ;
	dqv:expectedDataType xsd:float ;
	dqv:inDimension ex:completeness .
# 
# http://www.example.org#interpretability

ex:interpretability a owl:NamedIndividual , dqv:Dimension ;
	skos:definition "Interpretability covers a more technical aspect of information. It concerns the usage of appropriate languages, symbols and units. Interpretability can be enhanced by offering data conform best practices. It should also be noted that the more interpretable the data is, the easier it is to integrate it with other datasets."@en ;
	skos:prefLabel "Interpretability"@en ;
	dqv:inCategory ex:representation .
# 
# http://www.example.org#interpretabilityofdata

ex:interpretabilityofdata a owl:NamedIndividual , dqv:Metric ;
	ex:hasMetricType ex:DatasetQuality ;
	skos:definition "Detect the use of appropriate language, symbols, units and clear definitions. For instance, the use of abbreviations can make the dataset highly understandable, but its interpretation is limited to those who know the abbreviations."@en ;
	skos:prefLabel "Interpretability of Data"@en ;
	dqv:expectedDataType xsd:boolean ;
	dqv:inDimension ex:interpretability .
# 
# http://www.example.org#interpretabilityofterms

ex:interpretabilityofterms a owl:NamedIndividual , dqv:Metric ;
	ex:hasMetricType ex:DatasetQuality ;
	skos:definition "Use of various schema languages to provide definitions for terms. Providing definitions for used terms helps users to interpret the information. "@en ;
	skos:prefLabel "Interpretability of Terms"@en ;
	dqv:expectedDataType xsd:boolean ;
	dqv:inDimension ex:interpretability .
# 
# http://www.example.org#latency

ex:latency a owl:NamedIndividual , dqv:Metric ;
	ex:hasMetricType ex:DatasetQuality ;
	skos:definition "Latency is the delay between the submission of a request by a user, and the reception of a response from the system."@en ;
	skos:note "Unit of measure is milliseconds (ms)"@en ;
	skos:prefLabel "Latency"@en ;
	dqv:expectedDataType xsd:float ;
	dqv:inDimension ex:performance .
# 
# http://www.example.org#licencing

ex:licencing a owl:NamedIndividual , dqv:Dimension ;
	skos:definition "Concerns under which terms data can be (re)used."@en ;
	skos:prefLabel "Licencing"@en ;
	dqv:inCategory ex:accessibility .
# 
# http://www.example.org#machine-readablelicence

ex:machine-readablelicence a owl:NamedIndividual , dqv:Metric ;
	ex:hasMetricType ex:DatasetQuality ;
	skos:definition "Detection of the indication of a license in the VoID description or by means of dcterms:licence."@en ;
	skos:prefLabel "Machine-Readable Licence"@en ;
	dqv:expectedDataType xsd:boolean ;
	dqv:inDimension ex:licencing .
# 
# http://www.example.org#malformeddatatypeliterals

ex:malformeddatatypeliterals a owl:NamedIndividual , dqv:Metric ;
	ex:hasMetricType ex:InstanceQuality ;
	skos:definition "Measures the amount of literals with an unknown datatype."@en ;
	skos:prefLabel "Malformed Datatype Literals"@en ;
	dqv:expectedDataType xsd:integer ;
	dqv:inDimension ex:accuracy .
# 
# http://www.example.org#malformedtriples

ex:malformedtriples a owl:NamedIndividual , dqv:Metric ;
	ex:hasMetricType ex:SchemaQuality ;
	skos:definition "Detecting triples where the predicate is filled with an URI defined as a class or where the object position is filled by a property while the predicate is a rdf:type. These errors can be found with the help of a reasoner. "@en ;
	skos:prefLabel "Malformed Triples"@en ;
	dqv:expectedDataType xsd:integer ;
	dqv:inDimension ex:consistency .
# 
# http://www.example.org#meta-dataproperties

ex:meta-dataproperties a owl:NamedIndividual , dqv:Metric ;
	ex:hasMetricType ex:DatasetQuality ;
	skos:definition "measures the number of meta-data properties assigned to the dataset."@en ;
	skos:prefLabel "Meta-Data Properties"@en ;
	dqv:expectedDataType xsd:integer ;
	dqv:inDimension ex:relevancy .
# 
# http://www.example.org#meta-datasimilarity

ex:meta-datasimilarity a owl:NamedIndividual , dqv:Metric ;
	ex:hasMetricType ex:DatasetQuality ;
	skos:definition "By measuring the cosine similarity of 'descriptive' metadata (i.e. Description, theme, keywords/tags) between the two datasets, one can roughly assess whether one is relevant for the other. by using other information retrieval techniques (such as language modelling) one can deal with synomyny."@en ;
	skos:prefLabel "Meta-Data Similarity"@en ;
	dqv:expectedDataType xsd:float ;
	dqv:inDimension ex:relevancy .
# 
# http://www.example.org#objectivity

ex:objectivity a owl:NamedIndividual , dqv:Dimension ;
	skos:definition "The degree to which the interpretation and usage of data is unbiased, unprejudiced and impartial."@en ;
	skos:prefLabel "Objectivity"@en ;
	dqv:inCategory ex:trust .
# 
# http://www.example.org#ontologyhijacking

ex:ontologyhijacking a owl:NamedIndividual , dqv:Metric ;
	ex:hasMetricType ex:SchemaQuality ;
	skos:definition "Detection of the redefinition by third parties of classes/properties such that reasoning over data using those external terms is affected."@en ;
	skos:prefLabel "Ontology Hijacking"@en ;
	dqv:expectedDataType xsd:boolean ;
	dqv:inDimension ex:consistency .
# 
# http://www.example.org#outdatedinformation

ex:outdatedinformation a owl:NamedIndividual , dqv:Metric ;
	ex:hasMetricType ex:InstanceQuality ;
	skos:definition "With the usage of temporal metadata, one can (if available) detect outdated information based on the information retrieval concepts of age and freshness. By predicting the age of a resource, one can estimate when it should be updated. When a resource is overdue for an update, it can be considered outdated."@en ;
	skos:prefLabel "Outdated Information"@en ;
	dqv:expectedDataType xsd:float ;
	dqv:inDimension ex:currency .
# 
# http://www.example.org#outliers

ex:outliers a owl:NamedIndividual , dqv:Metric ;
	ex:hasMetricType ex:DataQuality ;
	skos:definition "<find consensus on measurement procedure>"@en ;
	skos:prefLabel "Outliers"@en ;
	dqv:expectedDataType xsd:integer ;
	dqv:inDimension ex:accuracy .
# 
# http://www.example.org#outwardlinks

ex:outwardlinks a owl:NamedIndividual , dqv:Metric ;
	ex:hasMetricType ex:DatasetQuality ;
	skos:definition "Detection of the existence and usage of external URIs and owl:sameAs links with external URIs."@en ;
	skos:prefLabel "Outward Links"@en ;
	dqv:expectedDataType xsd:boolean ;
	dqv:inDimension ex:interlinking .
# 
# http://www.example.org#performance

ex:performance a owl:NamedIndividual , dqv:Dimension ;
	skos:definition "Refers to the performance of a datasource and how well data can be accessed and processed."@en ;
	skos:prefLabel "Performance"@en ;
	dqv:inCategory ex:accessibility .
# 
# http://www.example.org#permissableusage

ex:permissableusage a owl:NamedIndividual , dqv:Metric ;
	ex:hasMetricType ex:DatasetQuality ;
	skos:definition "Detection of license indicating whether reproduction, distribution, modification or redistribution is permitted."@en ;
	skos:note "It is also possible for the Expected Data Type to be an URI, when available for the given licence"@en ;
	skos:prefLabel "Permissable Usage"@en ;
	dqv:expectedDataType xsd:string ;
	dqv:inDimension ex:licencing .
# 
# http://www.example.org#populationcompleteness

ex:populationcompleteness a owl:NamedIndividual , dqv:Metric ;
	ex:hasMetricType ex:DatasetQuality ;
	skos:definition "This metric measures the percentage of real-world objects represented in the dataset. Attaching a number to the amount of real-world object is a difficult task. In some cases it can be assumed that the primary dataset, approximately, contains the total amount of real-world objects. in this case the total amount of objects in the measure function is known. In other cases this number can be obtained by consulting other trusted data sources."@en ;
	skos:prefLabel "Population Completeness"@en ;
	dqv:expectedDataType xsd:float ;
	dqv:inDimension ex:completeness .
# 
# http://www.example.org#prefixindication

ex:prefixindication a owl:NamedIndividual , dqv:Metric ;
	ex:hasMetricType ex:DatasetQuality ;
	skos:definition "With the dataset, an indicaion of these external vocabularies should be provided to enhance understanding of the dataset. "@en ;
	skos:prefLabel "Prefix Indication"@en ;
	dqv:expectedDataType xsd:boolean ;
	dqv:inDimension ex:understandability .
# 
# http://www.example.org#prolixRDFfeatures

ex:prolixRDFfeatures a owl:NamedIndividual , dqv:Metric ;
	ex:hasMetricType ex:SchemaQuality ;
	skos:definition "Measure the usage of too lengthy rdf features such rdf reification, rdf containers and rdf collections. it is advised not to use these since it make the use of SPARQL more cumbersome and since the semantics behind these features are unclear."@en ;
	skos:prefLabel "Prolix RDF Features"@en ;
	dqv:expectedDataType xsd:boolean ;
	dqv:inDimension ex:representationalConciseness .
# 
# http://www.example.org#propertycompleteness

ex:propertycompleteness a owl:NamedIndividual , dqv:Metric ;
	ex:hasMetricType ex:InstanceQuality ;
	skos:definition "Property completeness entails every entity having the properties described in the schema known."@en ;
	skos:prefLabel "Property Completeness"@en ;
	dqv:expectedDataType xsd:float ;
	dqv:inDimension ex:completeness .
# 
# http://www.example.org#propertyconsistency

ex:propertyconsistency a owl:NamedIndividual , dqv:Metric ;
	ex:hasMetricType ex:SchemaQuality ;
	skos:definition "Measures the number of instances with identical values for different attributes. When two or more properties of an instance contains the same information, but with different naming, it could be redundant. "@en ;
	skos:prefLabel "Property Consistency"@en ;
	dqv:expectedDataType xsd:integer ;
	dqv:inDimension ex:consistency .
# 
# http://www.example.org#propertytype

ex:propertytype a owl:NamedIndividual , dqv:Metric ;
	ex:hasMetricType ex:SchemaQuality ;
	skos:definition "Properties of a resource can refer to either a literal value, or to a URI/blank-node, an owl:DatatypeProperty and a n owl:ObjectProperty, respectively. This metric measures the amount of triples where the datatype of the subject is incompatible with the predicate (property)."@en ;
	skos:prefLabel "Property Type"@en ;
	dqv:expectedDataType xsd:integer ;
	dqv:inDimension ex:consistency .
# 
# http://www.example.org#re-usedvocabularies

ex:re-usedvocabularies a owl:NamedIndividual , dqv:Metric ;
	ex:hasMetricType ex:SchemaQuality ;
	skos:definition "The usage of established vocabularies boosts the understandability (and uniformity) of the data schemas and thereby the ease of reuse. This metric measures the number of external vocabularies used."@en ;
	skos:prefLabel "Re-used Vocabularies"@en ;
	dqv:expectedDataType xsd:integer ;
	dqv:inDimension ex:representationalConsistency .
# 
# http://www.example.org#relevancy

ex:relevancy a owl:NamedIndividual , dqv:Dimension ;
	skos:definition "The extend to which information is applicable and helpful for a given task, and more specifically a query."@en ;
	skos:prefLabel "Relevancy"@en ;
	dqv:inCategory ex:contextual .
# 
# http://www.example.org#representationalConciseness

ex:representationalConciseness a owl:NamedIndividual , dqv:Dimension ;
	skos:definition "The extent to which the data is compact, clearly formatted and complete."@en ;
	skos:prefLabel "Representational Conciseness"@en ;
	dqv:inCategory ex:representation .
# 
# http://www.example.org#representationalConsistency

ex:representationalConsistency a owl:NamedIndividual , dqv:Dimension ;
	skos:definition "Representational-consistency is the degree to which the format and structure of the information conforms to previously returned information as well as data from other sources."@en ;
	skos:prefLabel "Representational Consistency"@en ;
	dqv:inCategory ex:representation .
# 
# http://www.example.org#reputation

ex:reputation a owl:NamedIndividual , dqv:Dimension ;
	skos:definition "Perceived trustworthiness of a dataset."@en ;
	skos:prefLabel "Reputation"@en ;
	dqv:inCategory ex:contextual , ex:trust .
# 
# http://www.example.org#reputationofdataset

ex:reputationofdataset a owl:NamedIndividual , dqv:Metric ;
	ex:hasMetricType ex:DatasetQuality ;
	skos:definition "By assigning explicit ratings to the dataset (manual) and analyzing external links or page rank (semi-automated)"@en ;
	skos:prefLabel "Reputation of Dataset"@en ;
	dqv:expectedDataType xsd:float ;
	dqv:inDimension ex:reputation .
# 
# http://www.example.org#resultsizerestriction

ex:resultsizerestriction a owl:NamedIndividual , dqv:Metric ;
	ex:hasMetricType ex:DatasetQuality ;
	skos:definition "Time-out errors can occur when the SPARQL query attempts to retrieve large amounts of data. Data providers can impose such restriction as well. The value for this metric is zero if no restriction is imposed."@en ;
	skos:note "The value of this metric is the max amount of results returned for a single query. If no restrictions are posed, the value is zero."@en ;
	skos:prefLabel "Result Size Restriction"@en ;
	dqv:expectedDataType xsd:integer ;
	dqv:inDimension ex:performance .
# 
# http://www.example.org#scalability

ex:scalability a owl:NamedIndividual , dqv:Metric ;
	ex:hasMetricType ex:DatasetQuality ;
	skos:definition "Detection of whether the time to answer an amount of ten requests divided by ten is not longer than the time it takes to answer one request."@en ;
	skos:prefLabel "Scalability"@en ;
	dqv:expectedDataType xsd:boolean ;
	dqv:inDimension ex:performance .
# 
# http://www.example.org#schemacompleteness

ex:schemacompleteness a owl:NamedIndividual , dqv:Metric ;
	ex:hasMetricType ex:SchemaQuality ;
	skos:definition "Usage of external (and established) vocabularies improves the machine-readability and reusability of a schema. They also provide an overview of properties and classes relevant for a given domain and scope. This metric measures the extend to which the vocabulary is exploited by taking the percentage of distinct classes and properties of an external vocabulary reused in the dataset.   "@en ;
	skos:prefLabel "Schema Completeness"@en ;
	dqv:expectedDataType xsd:float ;
	dqv:inDimension ex:completeness .
# 
# http://www.example.org#schemaenrichment

ex:schemaenrichment a owl:NamedIndividual , dqv:Metric ;
	ex:flags <http://www.opengis.net/ont/geosparql#Geometry> , <http://www.opengis.net/ont/geosparql#asWKT> , <http://www.opengis.net/ont/geosparql#hasGeometry> , rdf:type ;
	ex:hasMetricType ex:SchemaQuality ;
	skos:definition "Percentage of classes and properties reused from other sources."@en ;
	skos:prefLabel "Schema Enrichment"@en ;
	dqv:expectedDataType xsd:float ;
	dqv:inDimension ex:interlinking .
# 
# http://www.example.org#schemasimilarity

ex:schemasimilarity a owl:NamedIndividual , dqv:Metric ;
	ex:hasMetricType ex:SchemaQuality ;
	skos:definition "no. of classes and properties represented / total no. of classes and properties. for the purpose of interlinking, a more interesting form would take into account the intersection of the schema of both datasets as well as the parts only present in one of the datasets and their respective size."@en ;
	skos:note "Schema similarity metric annotates the number of classes and properties unique to each dataset and classes and properties shared by the datasets. The expected data type for this metrics depicts a 'similarity score' based on the previously mentioned amounts. "@en ;
	skos:prefLabel "Schema Similarity"@en ;
	dqv:expectedDataType xsd:float ;
	dqv:inDimension ex:completeness .
# 
# http://www.example.org#scope

ex:scope a owl:NamedIndividual ;
	ex:isPartOf ex:coverage ;
	skos:definition "Amount of entities represented in the dataset"@en ;
	skos:prefLabel "Scope"@en ;
	dqv:expectedDataType xsd:integer .
# 
# http://www.example.org#security

ex:security a owl:NamedIndividual , dqv:Dimension ;
	skos:definition "The extent to which (part of) the data is restricted from use, for instance when dealing with sensitive information."@en ;
	skos:prefLabel "Security"@en ;
	dqv:inCategory ex:accessibility .
# 
# http://www.example.org#serializationformats

ex:serializationformats a owl:NamedIndividual , dqv:Metric ;
	ex:hasMetricType ex:DatasetQuality ;
	skos:definition "Serialization formats such as turtle (which is a human-friendly serialization of rdf) and JSON-LD (an adaption of JSON) can both be used to publish a dataset and each is preferred for different use-cases. Having multiple serialization formats available lowers the threshold for users to use the dataset."@en ;
	skos:prefLabel "Serialization Formats"@en ;
	dqv:expectedDataType xsd:boolean ;
	dqv:inDimension ex:versatility .
# 
# http://www.example.org#slash-URIs

ex:slash-URIs a owl:NamedIndividual , dqv:Metric ;
	ex:hasMetricType ex:DatasetQuality ;
	skos:definition "Checking for usage of slash-URIs where large amounts of data is provided. The alternative would be 'hash-URIs', where the symbol before the last word is a hash. Hash-URIs have certain advantages when dealing with larger datasets in terms of performance. "@en ;
	skos:prefLabel "Slash-URIs"@en ;
	dqv:expectedDataType xsd:boolean ;
	dqv:inDimension ex:performance .
# 
# http://www.example.org#structureddata

ex:structureddata a owl:NamedIndividual , dqv:Metric ;
	ex:hasMetricType ex:DatasetQuality ;
	skos:definition "When the URI is dereferenceable, it should provide some useful structured information. The detection of dead links or URIs without any metadata or no redirection using the status code 303 See Other or no code 200 OK."@en ;
	skos:note "URIs not providing Structured data upon de-reference should be annotated. The proposed method is by means of the triple: <subject> ex:URLHasData 'False' "@en ;
	skos:prefLabel "Structured Data Availability"@en ;
	dqv:expectedDataType xsd:float ;
	dqv:inDimension ex:availability .
# 
# http://www.example.org#surfacearea

ex:surfacearea a owl:NamedIndividual , dqv:Metric ;
	ex:hasMetricType ex:InstanceQuality ;
	skos:definition "Instances with a spatial representation specified, by means of a polygon, should also make use of the following property: <https://data.pdok.nl/cbs/2015/vocab/oppervlakte> This metric measure the degree to which this is the case."@en ;
	skos:prefLabel "Surface Area"@en ;
	dqv:expectedDataType xsd:float ;
	dqv:inDimension ex:completeness .
# 
# http://www.example.org#test

ex:test a owl:NamedIndividual .
# 
# http://www.example.org#throughput

ex:throughput a owl:NamedIndividual , dqv:Metric ;
	ex:hasMetricType ex:DatasetQuality ;
	skos:definition "Throughput of the sources measures the amount of HTTP requests answered per second."@en ;
	skos:prefLabel "Throughput"@en ;
	dqv:expectedDataType xsd:float ;
	dqv:inDimension ex:performance .
# 
# http://www.example.org#timeliness

ex:timeliness a owl:NamedIndividual , dqv:Dimension ;
	skos:definition "Timeliness measures how up-to-data data is, relative to a specific task."@en ;
	skos:prefLabel "Timeliness"@en ;
	dqv:inCategory ex:datasetdynamicity , ex:intrinsic .
# 
# http://www.example.org#timelinessideal

ex:timelinessideal a owl:NamedIndividual , dqv:Metric ;
	ex:hasMetricType ex:DatasetQuality ;
	skos:definition "Ideally, both datasets would be equally fresh, especially with highly volatile data. Differences in freshness could result in inconsistencies even though, at time of publication, each dataset was flawless. This metric measures the difference between the ideal freshness (freshness of the primary dataset) and the freshness of the Target dataset."@en ;
	skos:prefLabel "Timeliness Ideal"@en ;
	dqv:expectedDataType xsd:dayTimeDuration ;
	dqv:inDimension ex:timeliness .
# 
# http://www.example.org#timelinessofdatasource

ex:timelinessofdatasource a owl:NamedIndividual , dqv:Metric ;
	ex:hasMetricType ex:DatasetQuality ;
	skos:definition "This metric measures the delay with which the semantic source is updated in regard to its original source, if present. "@en ;
	skos:prefLabel "Timeliness of Datasource"@en ;
	dqv:expectedDataType xsd:dayTimeDuration ;
	dqv:inDimension ex:timeliness .
# 
# http://www.example.org#timelinessofresource

ex:timelinessofresource a owl:NamedIndividual , dqv:Metric ;
	ex:hasMetricType ex:InstanceQuality ;
	skos:definition "A positive difference between current and expiry time of the resource implies data source to be outdated"@en ;
	skos:prefLabel "Timeliness of Resource"@en ;
	dqv:expectedDataType xsd:dayTimeDuration ;
	dqv:inDimension ex:timeliness .
# 
# http://www.example.org#timesincelastmodification

ex:timesincelastmodification a owl:NamedIndividual , dqv:Metric ;
	ex:hasMetricType ex:DatasetQuality ;
	skos:definition "Time since last modification"@en ;
	skos:prefLabel "Time Since Last Modification"@en ;
	dqv:expectedDataType xsd:dayTimeDuration ;
	dqv:inDimension ex:currency .
# 
# http://www.example.org#undefinedclasses

ex:undefinedclasses a owl:NamedIndividual , dqv:Metric ;
	ex:hasMetricType ex:SchemaQuality ;
	skos:definition "Measured usage of undefined classes"@en ;
	skos:prefLabel "Undefined Classes"@en ;
	dqv:expectedDataType xsd:integer ;
	dqv:inDimension ex:consistency .
# 
# http://www.example.org#undefinedproperties

ex:undefinedproperties a owl:NamedIndividual , dqv:Metric ;
	ex:hasMetricType ex:SchemaQuality ;
	skos:definition "Measured usage of undefined properties"@en ;
	skos:prefLabel "Undefined Properties"@en ;
	dqv:expectedDataType xsd:integer ;
	dqv:inDimension ex:consistency .
# 
# http://www.example.org#understandability

ex:understandability a owl:NamedIndividual , dqv:Dimension ;
	skos:definition "The ease with which data can be comprehended, without ambiguity, and used."@en ;
	skos:prefLabel "Understandability"@en ;
	dqv:inCategory ex:representation .
# 
# http://www.example.org#uniformspatialrepresentation

ex:uniformspatialrepresentation a owl:NamedIndividual , dqv:Metric ;
	ex:hasMetricType ex:InstanceQuality ;
	skos:definition "Uniformity in datatype for  geometry is measured for this metric. This metric checks whether every geometry is of a specific datatype."@en ;
	skos:prefLabel "Uniform Spatial Representation"@en ;
	dqv:expectedDataType xsd:float ;
	dqv:inDimension ex:representationalConsistency .
# 
# http://www.example.org#validitytimeinterval

ex:validitytimeinterval a owl:NamedIndividual , dqv:Metric ;
	ex:hasMetricType ex:DataQuality ;
	skos:definition "Given that an expiry time is known, a validity interval can be computed based on the time of input and the expiry date. If no expiry time is provided, a measure used in Metric <Exclusion of outdated data> can be used to calculate when the dataset is due for an update. However, this alternative would not measure validity as strictly and instead would measure 'likeliness of being up to date' and hence valid."@en ;
	skos:prefLabel "Validity Time Interval"@en ;
	dqv:expectedDataType xsd:date ;
	dqv:inDimension ex:volatility .
# 
# http://www.example.org#verifiability

ex:verifiability a owl:NamedIndividual , dqv:Dimension ;
	skos:definition "The ease with which the data can be assessed for correctness."@en ;
	skos:prefLabel "Verifiability"@en ;
	dqv:inCategory ex:contextual , ex:trust .
# 
# http://www.example.org#versatility

ex:versatility a owl:NamedIndividual , dqv:Dimension ;
	skos:definition "The availability of alternative representations and access methods."@en ;
	skos:prefLabel "Versatility"@en ;
	dqv:inCategory ex:representation .
# 
# http://www.example.org#vocabularysimilarity

ex:vocabularysimilarity a owl:NamedIndividual , dqv:Metric ;
	ex:hasMetricType ex:SchemaQuality ;
	skos:definition "Interlinking datasets that use different notations for identical information can convolute the process. If both datasets use a vocabulary, it can provide junctions where the two datasets can be interlinked."@en ;
	skos:prefLabel "Vocabulary Similarity"@en ;
	dqv:expectedDataType xsd:integer ;
	dqv:inDimension ex:representationalConsistency .
# 
# http://www.example.org#voidvalues

ex:voidvalues a owl:NamedIndividual , dqv:Metric ;
	ex:hasMetricType ex:SchemaQuality ;
	skos:definition "Usage owl:Inverse-functionalProperty implies a resource can be uniquely identified by the value of the property. When this usage results in faulty values (void values), it will no longer uniquely identify a resource, but each resource with a similar void value, resulting in an explosion of owl:sameAs links."@en ;
	skos:note "void values should be listed and respective instances annotated."@en ;
	skos:prefLabel "Void Values"@en ;
	dqv:expectedDataType xsd:integer ;
	dqv:inDimension ex:consistency .
# 
# http://www.example.org#volatility

ex:volatility a owl:NamedIndividual , dqv:Dimension ;
	skos:definition "The frequency of changes in the data over time."@en ;
	skos:prefLabel "Volatility"@en ;
	dqv:inCategory ex:datasetdynamicity .
